erc20_pausable: move inrange assumptions to the model definition

erc20_pausable/DSL.v
@@ -418,6 +418,17 @@ Notation "'@string' x = expr ; stmt" :=
 
 Require Import Spec.
 
+Definition dsl_sat_spec (fcall: mcall)
+                        (fdsl: Stmt)
+                        (fspec: address -> env -> message -> Spec) : Prop :=
+  forall st env msg this,
+    m_func msg = fcall
+    -> spec_require (fspec this env msg) st
+    -> forall st0 result,
+      dsl_exec fdsl st0 st env msg this nil = result
+      -> spec_trans (fspec this env msg) st (ret_st result)
+         /\ spec_events (fspec this env msg) (ret_st result) (ret_evts result).
+
 Section dsl_transfer_from.
   Open Scope dsl_scope.
 
@@ -435,7 +446,6 @@ Section dsl_transfer_from.
   Context `{from_immutable: forall st env msg, from st env msg = _from}.
   Context `{to_immutable: forall st env msg, to st env msg = _to}.
   Context `{value_immutable: forall st env msg, value st env msg = _value}.
-  Context `{value_in_range: (_value >= 0 /\ _value <= MAX_UINT256)%nat}.
   Context `{max_uint256_immutable: forall st env msg, max_uint256 st env msg = MAX_UINT256}.
 
   (* DSL representation of transferFrom(), generated from solidity *)
@@ -458,11 +468,15 @@ Section dsl_transfer_from.
   (* Auxiliary lemmas *)
   Lemma nat_nooverflow_dsl_nooverflow:
     forall (m: state -> a2v) st env msg,
+      m_func msg = mc_transferFrom _from _to _value ->
       (_from = _to \/ (_from <> _to /\ (m st _to <= MAX_UINT256 - _value)))%nat ->
       ((from == to) ||
        ((fun st env msg => m st (to st env msg)) <= max_uint256 - value))%dsl st env msg = otrue.
   Proof.
-    intros m st env msg Hnat.
+    intros m st env msg Hmcall Hnat.
+
+    apply transferFrom_value_inrange in Hmcall.
+    destruct Hmcall as [_ Hvalue].
 
     unfold "=="%dsl, "<="%dsl, "||"%dsl, "||"%bool, "-"%dsl.
     rewrite (from_immutable st env msg),
@@ -474,28 +488,74 @@ Section dsl_transfer_from.
     - destruct H as [Hneq Hle].
       apply Nat.eqb_neq in Hneq. rewrite Hneq.
       apply Nat.leb_le in Hle.
-      destruct value_in_range as [_ Hvalue].
       assert (Hlo: (MAX_UINT256 >= _value)%nat);
         auto.
       rewrite (minus_safe _ _ Hlo).
       exact Hle.
   Qed.
 
+  Lemma transferFrom_cond_dec:
+    forall st,
+      Decidable.decidable
+        (_from = _to \/ _from <> _to /\ (st_balances st _to <= MAX_UINT256 - _value)%nat).
+  Proof.
+    intros.
+    apply Decidable.dec_or.
+    - apply Nat.eq_decidable.
+    - apply Decidable.dec_and.
+      + apply neq_decidable.
+      + apply Nat.le_decidable.
+  Qed.
+
+  Lemma transferFrom_cond_impl:
+    forall st env msg,
+      m_func msg = mc_transferFrom _from _to _value ->
+      ~ (_from = _to \/ _from <> _to /\ (st_balances st _to <= MAX_UINT256 - _value)%nat) ->
+      (((from == to)
+        || ((fun (st : state) (env : Model.env) (msg : message) =>
+               st_balances st (to st env msg)) <= max_uint256 - value)) st env msg) = ofalse.
+  Proof.
+    intros st env msg Hfunc Hneg.
+
+    apply transferFrom_value_inrange in Hfunc.
+    destruct Hfunc as [_ Hvalue].
+
+    unfold "=="%dsl, "||"%dsl, "||"%bool, "<="%dsl, "-"%dsl.
+    rewrite (from_immutable _ _ _).
+    rewrite (to_immutable _ _ _).
+    rewrite (value_immutable _ _ _).
+    rewrite (max_uint256_immutable _ _ _).
+
+    apply (Decidable.not_or _ _) in Hneg.
+    destruct Hneg as [Hneq Hneg].
+
+    apply Nat.eqb_neq in Hneq.
+    rewrite Hneq; simpl.
+
+    assert (Hvalue': (MAX_UINT256 >= _value)%nat);
+      auto.
+    rewrite (minus_safe _ _ Hvalue').
+
+    apply (Decidable.not_and _ _ (neq_decidable _ _)) in Hneg.
+    destruct Hneg.
+    - apply Nat.eqb_neq in Hneq. apply H in Hneq. inversion Hneq.
+    - apply not_le in H.
+      apply Nat.leb_gt.
+      auto.
+  Qed.
+
   (* Manually proved *)
   Lemma transferFrom_dsl_sat_spec_1:
-    forall st env msg this,
-      spec_require (funcspec_transferFrom_1 _from _to _value this env msg) st ->
-      forall st0 result,
-        dsl_exec transferFrom_dsl st0 st env msg this nil = result ->
-        spec_trans (funcspec_transferFrom_1 _from _to _value this env msg) st (ret_st result) /\
-        spec_events (funcspec_transferFrom_1 _from _to _value this env msg) (ret_st result) (ret_evts result).
+    dsl_sat_spec (mc_transferFrom _from _to _value)
+                 transferFrom_dsl
+                 (funcspec_transferFrom_1 _from _to _value).
   Proof.
-    intros st env msg this Hreq st0 result Hexec.
+    intros st env msg this Hfunc Hreq st0 result Hexec.
 
     simpl in Hreq.
     destruct Hreq as [Hpaused [Hreq_blncs_lo [Hreq_blncs_hi [Hreq_allwd_lo Hreq_allwd_hi]]]].
     apply Nat.leb_le in Hreq_blncs_lo.
-    generalize (nat_nooverflow_dsl_nooverflow _ st env msg Hreq_blncs_hi).
+    generalize (nat_nooverflow_dsl_nooverflow _ st env msg Hfunc Hreq_blncs_hi).
     clear Hreq_blncs_hi. intros Hreq_blncs_hi.
     apply Nat.leb_le in Hreq_allwd_lo.
     apply Nat.ltb_lt in Hreq_allwd_hi.
@@ -537,17 +597,14 @@ Section dsl_transfer_from.
   Qed.
 
   Lemma transferFrom_dsl_sat_spec_2:
-    forall st env msg this,
-      spec_require (funcspec_transferFrom_2 _from _to _value this env msg) st ->
-      forall st0 result,
-        dsl_exec transferFrom_dsl st0 st env msg this nil = result ->
-        spec_trans (funcspec_transferFrom_2 _from _to _value this env msg) st (ret_st result) /\
-        spec_events (funcspec_transferFrom_2 _from _to _value this env msg) (ret_st result) (ret_evts result).
+    dsl_sat_spec (mc_transferFrom _from _to _value)
+                 transferFrom_dsl
+                 (funcspec_transferFrom_2 _from _to _value).
   Proof.
-    intros st env msg this Hreq st0 result Hexec.
+    intros st env msg this Hfunc Hreq st0 result Hexec.
 
     simpl in Hreq. destruct Hreq as [Hpaused [Hreq_blncs_lo [Hreq_blncs_hi [Hreq_allwd_lo Hreq_allwd_hi]]]].
-    generalize (nat_nooverflow_dsl_nooverflow _ st env msg Hreq_blncs_hi).
+    generalize (nat_nooverflow_dsl_nooverflow _ st env msg Hfunc Hreq_blncs_hi).
     clear Hreq_blncs_hi. intros Hreq_blncs_hi.
     apply Nat.leb_le in Hreq_blncs_lo.
     apply Nat.leb_le in Hreq_allwd_lo.
@@ -589,56 +646,10 @@ Section dsl_transfer_from.
     repeat (split; auto).
   Qed.
 
-  Lemma transferFrom_cond_dec:
-    forall st,
-      Decidable.decidable
-        (_from = _to \/ _from <> _to /\ (st_balances st _to <= MAX_UINT256 - _value)%nat).
-  Proof.
-    intros.
-    apply Decidable.dec_or.
-    - apply Nat.eq_decidable.
-    - apply Decidable.dec_and.
-      + apply neq_decidable.
-      + apply Nat.le_decidable.
-  Qed.
-
-  Lemma transferFrom_cond_impl:
-    forall st env msg,
-      ~ (_from = _to \/ _from <> _to /\ (st_balances st _to <= MAX_UINT256 - _value)%nat) ->
-      (((from == to)
-        || ((fun (st : state) (env : Model.env) (msg : message) =>
-               st_balances st (to st env msg)) <= max_uint256 - value)) st env msg) = ofalse.
-  Proof.
-    intros st env msg Hneg.
-
-    unfold "=="%dsl, "||"%dsl, "||"%bool, "<="%dsl, "-"%dsl.
-    rewrite (from_immutable _ _ _).
-    rewrite (to_immutable _ _ _).
-    rewrite (value_immutable _ _ _).
-    rewrite (max_uint256_immutable _ _ _).
-
-    apply (Decidable.not_or _ _) in Hneg.
-    destruct Hneg as [Hneq Hneg].
-
-    apply Nat.eqb_neq in Hneq.
-    rewrite Hneq; simpl.
-
-    destruct value_in_range as [_ Hvalue].
-    assert (Hvalue': (MAX_UINT256 >= _value)%nat);
-      auto.
-    rewrite (minus_safe _ _ Hvalue').
-
-    apply (Decidable.not_and _ _ (neq_decidable _ _)) in Hneg.
-    destruct Hneg.
-    - apply Nat.eqb_neq in Hneq. apply H in Hneq. inversion Hneq.
-    - apply not_le in H.
-      apply Nat.leb_gt.
-      auto.
-  Qed.
-
   (* If no require can be satisfied, transferFrom() must revert to the initial state *)
   Lemma transferFrom_dsl_revert:
     forall st env msg this,
+      m_func msg = mc_transferFrom _from _to _value ->
       ~ spec_require (funcspec_transferFrom_1 _from _to _value this env msg) st ->
       ~ spec_require (funcspec_transferFrom_2 _from _to _value this env msg) st ->
       (forall addr0 addr1, (st_allowed st (addr0, addr1) <= MAX_UINT256)%nat) ->
@@ -647,7 +658,7 @@ Section dsl_transfer_from.
         result = Stop st0 (ev_revert this :: nil).
   Proof.
     unfold funcspec_transferFrom_1, funcspec_transferFrom_2, ">="%nat.
-    intros st env msg this Hreq1_neg Hreq2_neg Hallwd_inv st0 result Hexec;
+    intros st env msg this Hfunc Hreq1_neg Hreq2_neg Hallwd_inv st0 result Hexec;
       simpl in Hreq1_neg, Hreq2_neg.
 
     assert (Hreq1_impl:
@@ -767,7 +778,7 @@ Section dsl_transfer_from.
             }
             clear Hreq2_impl; rename Himpl into Hreq2_impl.
 
-            generalize (nat_nooverflow_dsl_nooverflow _ _ env msg H); intros Hcond.
+            generalize (nat_nooverflow_dsl_nooverflow _ _ env msg Hfunc H); intros Hcond.
             unfold dsl_allowed_access in Hexec.
             rewrite Hcond in Hexec; simpl in Hexec; clear Hcond.
 
@@ -805,7 +816,7 @@ Section dsl_transfer_from.
               split; auto.
 
           + (* from <> to /\ balances[to] >= MAX_UINT256 + value *)
-            apply (transferFrom_cond_impl st env msg) in H.
+            apply (transferFrom_cond_impl st env msg Hfunc) in H.
             rewrite H in Hexec; simpl in Hexec.
 
             rewrite <- Hexec.
@@ -850,7 +861,6 @@ Section dsl_transfer.
   (* Arguments are immutable, generated from solidity *)
   Context `{to_immutable: forall st env msg, to st env msg = _to}.
   Context `{value_immutable: forall st env msg, value st env msg = _value}.
-  Context `{value_in_range: (_value >= 0 /\ _value <= MAX_UINT256)%nat}.
   Context `{max_uint256_immutable: forall st env msg, max_uint256 st env msg = MAX_UINT256}.
 
   (* DSL representation of transfer(), generated from solidity *)
@@ -867,11 +877,15 @@ Section dsl_transfer.
   (* Auxiliary lemmas *)
   Lemma nat_nooverflow_dsl_nooverflow':
     forall (m: state -> a2v) st env msg,
+      m_func msg = mc_transfer _to _value ->
       (m_sender msg = _to \/ (m_sender msg <> _to /\ (m st _to <= MAX_UINT256 - _value)))%nat ->
       ((msg.sender == to) ||
        ((fun st env msg => m st (to st env msg)) <= max_uint256 - value))%dsl st env msg = otrue.
   Proof.
-    intros m st env msg Hnat.
+    intros m st env msg Hfunc Hnat.
+
+    apply transfer_value_inrange in Hfunc.
+    destruct Hfunc as [_ Hvalue].
 
     unfold "||"%dsl, "||"%bool, "=="%dsl, "<="%dsl, "-"%dsl.
     rewrite (to_immutable st env msg),
@@ -881,28 +895,58 @@ Section dsl_transfer.
     - rewrite H. rewrite (Nat.eqb_refl _). reflexivity.
     - destruct H as [Hneq Hle].
       apply Nat.eqb_neq in Hneq. rewrite Hneq.
-      destruct value_in_range as [_ Hvalue].
       assert (Hlo: (MAX_UINT256 >= _value)%nat);
         auto.
       rewrite (minus_safe _ _ Hlo).
       apply Nat.leb_le in Hle. exact Hle.
   Qed.
 
+  Lemma transfer_cond_impl:
+    forall st env msg,
+      m_func msg = mc_transfer _to _value ->
+      m_sender msg <> _to /\
+      ~ (m_sender msg <> _to /\ (st_balances st _to <= MAX_UINT256 - _value)%nat) ->
+      (((fun (_ : state) (_ : Model.env) (msg : message) => m_sender msg) == to)
+       || ((fun (st : state) (env : Model.env) (msg : message) =>
+              st_balances st (to st env msg)) <= max_uint256 - value)) st env msg = ofalse.
+  Proof.
+    intros st env msg Hfunc Hcond.
+
+    apply transfer_value_inrange in Hfunc.
+    destruct Hfunc as [_ Hvalue].
+
+    unfold "=="%dsl, "||"%dsl, "||"%bool, "<="%dsl, "-"%dsl.
+    rewrite (value_immutable _ _ _).
+    rewrite (to_immutable _ _ _).
+    rewrite (max_uint256_immutable _ _ _).
+    rewrite (minus_safe _ _ Hvalue).
+
+    destruct Hcond as [Hneq Heq].
+    apply Nat.eqb_neq in Hneq; rewrite Hneq; simpl.
+
+    apply (Decidable.not_and _ _ (neq_decidable _ _)) in Heq.
+    destruct Heq.
+
+    - apply Nat.eqb_neq in Hneq.
+      apply H in Hneq; inversion Hneq.
+
+    - apply not_le in H.
+      apply Nat.leb_gt.
+      auto.
+  Qed.
+
   (* Manually proved *)
   Lemma transfer_dsl_sat_spec:
-    forall st env msg this,
-      spec_require (funcspec_transfer _to _value this env msg) st ->
-      forall st0 result,
-        dsl_exec transfer_dsl st0 st env msg this nil = result ->
-        spec_trans (funcspec_transfer _to _value this env msg) st (ret_st result) /\
-        spec_events (funcspec_transfer _to _value this env msg) (ret_st result) (ret_evts result).
+    dsl_sat_spec (mc_transfer _to _value)
+                 transfer_dsl
+                 (funcspec_transfer _to _value).
   Proof.
-    intros st env msg this Hreq st0 result Hexec.
+    intros st env msg this Hfunc Hreq st0 result Hexec.
 
     unfold funcspec_transfer in Hreq; simpl in Hreq.
     destruct Hreq as [Hpaused [Hreq_blncs_lo Hreq_blncs_hi]].
     unfold ">="%nat in Hreq_blncs_lo. apply Nat.leb_le in Hreq_blncs_lo.
-    generalize(nat_nooverflow_dsl_nooverflow' _ st env msg Hreq_blncs_hi).
+    generalize(nat_nooverflow_dsl_nooverflow' _ st env msg Hfunc Hreq_blncs_hi).
     clear Hreq_blncs_hi. intros Hreq_blncs_hi.
 
     unfold transfer_dsl in Hexec; simpl in Hexec.
@@ -924,46 +968,16 @@ Section dsl_transfer.
     repeat (split; auto).
   Qed.
 
-  Lemma transfer_cond_impl:
-    forall st env msg,
-      m_sender msg <> _to /\
-      ~ (m_sender msg <> _to /\ (st_balances st _to <= MAX_UINT256 - _value)%nat) ->
-      (((fun (_ : state) (_ : Model.env) (msg : message) => m_sender msg) == to)
-       || ((fun (st : state) (env : Model.env) (msg : message) =>
-              st_balances st (to st env msg)) <= max_uint256 - value)) st env msg = ofalse.
-  Proof.
-    intros st env msg Hcond.
-
-    unfold "=="%dsl, "||"%dsl, "||"%bool, "<="%dsl, "-"%dsl.
-    rewrite (value_immutable _ _ _).
-    rewrite (to_immutable _ _ _).
-    rewrite (max_uint256_immutable _ _ _).
-    destruct value_in_range as [_ Hvalue].
-    rewrite (minus_safe _ _ Hvalue).
-
-    destruct Hcond as [Hneq Heq].
-    apply Nat.eqb_neq in Hneq; rewrite Hneq; simpl.
-
-    apply (Decidable.not_and _ _ (neq_decidable _ _)) in Heq.
-    destruct Heq.
-
-    - apply Nat.eqb_neq in Hneq.
-      apply H in Hneq; inversion Hneq.
-
-    - apply not_le in H.
-      apply Nat.leb_gt.
-      auto.
-  Qed.
-
   (* If no require can be satisfied, transfer() must revert to the initial state *)
   Lemma transfer_dsl_revert:
     forall st env msg this,
+      m_func msg = mc_transfer _to _value ->
       ~ spec_require (funcspec_transfer _to _value this env msg) st ->
       forall st0 result,
         dsl_exec transfer_dsl st0 st env msg this nil = result ->
         result = Stop st0 (ev_revert this :: nil).
   Proof.
-    intros st env msg this Hreq_neg st0 result Hexec.
+    intros st env msg this Hfunc Hreq_neg st0 result Hexec.
 
     simpl in Hreq_neg.
 
@@ -1011,7 +1025,7 @@ Section dsl_transfer.
           rewrite (Nat.ltb_antisym _ _) in Hexec.
           rewrite l in Hexec; simpl in Hexec.
 
-          apply (transfer_cond_impl st env msg)in Hreq.
+          apply (transfer_cond_impl st env msg Hfunc)in Hreq.
           rewrite Hreq in Hexec; clear Hreq; simpl in Hexec.
 
           rewrite <- Hexec.
@@ -1059,14 +1073,11 @@ Section dsl_balanceOf.
 
   (* Manually proved *)
   Lemma balanceOf_dsl_sat_spec:
-    forall st env msg this,
-      spec_require (funcspec_balanceOf __owner this env msg) st ->
-      forall st0 result,
-        dsl_exec balanceOf_dsl st0 st env msg this nil = result ->
-        spec_trans (funcspec_balanceOf __owner this env msg) st (ret_st result) /\
-        spec_events (funcspec_balanceOf __owner this env msg) (ret_st result) (ret_evts result).
+    dsl_sat_spec (mc_balanceOf __owner)
+                 balanceOf_dsl
+                 (funcspec_balanceOf __owner).
   Proof.
-    intros st env msg this Hreq st0 result Hexec.
+    intros st env msg this Hfunc Hreq st0 result Hexec.
 
     simpl in Hexec.
     unfold funcspec_balanceOf.
@@ -1079,12 +1090,13 @@ Section dsl_balanceOf.
   (* If no require can be satisfied, balanceOf() must revert to the initial state *)
   Lemma balanceOf_dsl_revert:
     forall st env msg this,
+      m_func msg = mc_balanceOf __owner ->
       ~ spec_require (funcspec_balanceOf __owner this env msg) st ->
       forall st0 result,
         dsl_exec balanceOf_dsl st0 st env msg this nil = result ->
         result = Stop st0 (ev_revert this :: nil).
   Proof.
-    intros st env msg this Hreq_neg st0 result Hexec.
+    intros st env msg this _ Hreq_neg st0 result Hexec.
     simpl in Hreq_neg.
     apply (proj1 Decidable.not_true_iff) in Hreq_neg.
     inversion Hreq_neg.
@@ -1116,14 +1128,11 @@ Section dsl_approve.
 
   (* Manually proved *)
   Lemma approve_dsl_sat_spec:
-    forall st env msg this,
-      spec_require (funcspec_approve _spender _value this env msg) st ->
-      forall st0 result,
-        dsl_exec approve_dsl st0 st env msg this nil = result ->
-        spec_trans (funcspec_approve _spender _value this env msg) st (ret_st result) /\
-        spec_events (funcspec_approve _spender _value this env msg) (ret_st result) (ret_evts result).
+    dsl_sat_spec (mc_approve _spender _value)
+                 approve_dsl
+                 (funcspec_approve _spender _value).
   Proof.
-    intros st env msg this Hreq st0 result Hexec.
+    intros st env msg this Hfunc Hreq st0 result Hexec.
 
     simpl in Hreq.
     simpl in Hexec.
@@ -1138,12 +1147,13 @@ Section dsl_approve.
   (* If no require can be satisfied, approve() must revert to the initial state *)
   Lemma approve_dsl_revert:
     forall st env msg this,
+      m_func msg = mc_approve _spender _value ->
       ~ spec_require (funcspec_approve _spender _value this env msg) st ->
       forall st0 result,
         dsl_exec approve_dsl st0 st env msg this nil = result ->
         result = Stop st0 (ev_revert this :: nil).
   Proof.
-    intros st env msg this Hreq_neg st0 result Hexec.
+    intros st env msg this Hfunc Hreq_neg st0 result Hexec.
 
     simpl in Hreq_neg.
     apply not_false_is_true in Hreq_neg.
@@ -1177,14 +1187,11 @@ Section dsl_allowance.
 
   (* Manually proved *)
   Lemma allowance_dsl_sat_spec:
-    forall st env msg this,
-      spec_require (funcspec_allowance __owner _spender this env msg) st ->
-      forall st0 result,
-        dsl_exec allowance_dsl st0 st env msg this nil = result ->
-        spec_trans (funcspec_allowance __owner _spender this env msg) st (ret_st result) /\
-        spec_events (funcspec_allowance __owner _spender this env msg) (ret_st result) (ret_evts result).
+    dsl_sat_spec (mc_allowance __owner _spender)
+                 allowance_dsl
+                 (funcspec_allowance __owner _spender).
   Proof.
-    intros st env msg this Hreq st0 result Hexec.
+    intros st env msg this Hfunc Hreq st0 result Hexec.
 
     simpl in Hexec.
     unfold funcspec_allowance.
@@ -1198,12 +1205,13 @@ Section dsl_allowance.
   (* If no require can be satisfied, allowance() must revert to the initial state *)
   Lemma allowance_dsl_revert:
     forall st env msg this,
+      m_func msg = mc_allowance __owner _spender ->
       ~ spec_require (funcspec_allowance __owner _spender this env msg) st ->
       forall st0 result,
         dsl_exec allowance_dsl st0 st env msg this nil = result ->
         result = Stop st0 (ev_revert this :: nil).
   Proof.
-    intros st env msg this Hreq_neg st0 result Hexec.
+    intros st env msg this Hfunc Hreq_neg st0 result Hexec.
     simpl in Hreq_neg.
     apply (proj1 Decidable.not_true_iff) in Hreq_neg.
     inversion Hreq_neg.
@@ -1249,13 +1257,14 @@ Section dsl_constructor.
       st_balances st = $0 ->
       st_allowed st = $0 ->
       forall env msg this,
+        m_func msg = mc_PausableToken _initialAmount _tokenName _decimalUnits _tokenSymbol ->
         spec_require (funcspec_PausableToken _initialAmount _tokenName _decimalUnits _tokenSymbol this env msg) st ->
         forall st0 result,
           dsl_exec ctor_dsl st0 st env msg this nil = result ->
           spec_trans (funcspec_PausableToken _initialAmount _tokenName _decimalUnits _tokenSymbol this env msg) st (ret_st result) /\
           spec_events (funcspec_PausableToken _initialAmount _tokenName _decimalUnits _tokenSymbol this env msg) (ret_st result) (ret_evts result).
   Proof.
-    intros st Hblns_init Hallwd_init env msg this Hreq st0 result Hexec.
+    intros st Hblns_init Hallwd_init env msg this Hfunc Hreq st0 result Hexec.
 
     simpl in Hexec.
     unfold funcspec_PausableToken.
@@ -1285,14 +1294,11 @@ Section dsl_pause.
 
   (* Manually proved *)
   Lemma pause_dsl_sat_spec:
-    forall st env msg this,
-      spec_require (funcspec_pause this env msg) st ->
-      forall st0 result,
-        dsl_exec pause_dsl st0 st env msg this nil = result ->
-        spec_trans (funcspec_pause this env msg) st (ret_st result) /\
-        spec_events (funcspec_pause this env msg) (ret_st result) (ret_evts result).
+    dsl_sat_spec mc_pause
+                 pause_dsl
+                 funcspec_pause.
   Proof.
-    intros st env msg this Hreq st0 result Hexec.
+    intros st env msg this Hfunc Hreq st0 result Hexec.
 
     simpl in Hreq.
     destruct Hreq as [Hpause Howner].
@@ -1311,12 +1317,13 @@ Section dsl_pause.
   (* If no require can be satisfied, pause() must revert to the initial state *)
   Lemma pause_dsl_revert:
     forall st env msg this,
+      m_func msg = mc_pause ->
       ~ spec_require (funcspec_pause this env msg) st ->
       forall st0 result,
         dsl_exec pause_dsl st0 st env msg this nil = result ->
         result = Stop st0 (ev_revert this :: nil).
   Proof.
-    intros st env msg this Hreq_neg st0 result Hexec.
+    intros st env msg this Hfunc Hreq_neg st0 result Hexec.
 
     simpl in Hreq_neg.
     assert (Hreq_impl: st_paused st = ofalse -> ~ st_owner st = m_sender msg).
@@ -1369,14 +1376,11 @@ Section dsl_unpause.
 
   (* Manually proved *)
   Lemma unpause_dsl_sat_spec:
-    forall st env msg this,
-      spec_require (funcspec_unpause this env msg) st ->
-      forall st0 result,
-        dsl_exec unpause_dsl st0 st env msg this nil = result ->
-        spec_trans (funcspec_unpause this env msg) st (ret_st result) /\
-        spec_events (funcspec_unpause this env msg) (ret_st result) (ret_evts result).
+    dsl_sat_spec mc_unpause
+                 unpause_dsl
+                 funcspec_unpause.
   Proof.
-    intros st env msg this Hreq st0 result Hexec.
+    intros st env msg this Hfunc Hreq st0 result Hexec.
 
     simpl in Hreq.
     destruct Hreq as [Hpause Howner].
@@ -1394,12 +1398,13 @@ Section dsl_unpause.
   (* If no require can be satisfied, unpause() must revert to the initial state *)
   Lemma unpause_dsl_revert:
     forall st env msg this,
+      m_func msg = mc_unpause ->
       ~ spec_require (funcspec_unpause this env msg) st ->
       forall st0 result,
         dsl_exec unpause_dsl st0 st env msg this nil = result ->
         result = Stop st0 (ev_revert this :: nil).
   Proof.
-    intros st env msg this Hreq_neg st0 result Hexec.
+    intros st env msg this Hfunc Hreq_neg st0 result Hexec.
 
     simpl in Hreq_neg.
     assert (Hreq_impl: st_paused st = otrue -> ~ st_owner st = m_sender msg).
@@ -1452,7 +1457,6 @@ Section dsl_increaseApproval.
   (* Arguments are immutable, generated from solidity *)
   Context `{spender_immutable: forall st env msg, spender st env msg = _spender}.
   Context `{value_immutable: forall st env msg, value st env msg = _value}.
-  Context `{value_in_range: (0 <= _value /\ _value <= MAX_UINT256)%nat}.
   Context `{max_uint256_immutable: forall st env msg, max_uint256 st env msg = MAX_UINT256}.
 
   (* DSL representation of constructor, generated from solidity *)
@@ -1465,14 +1469,14 @@ Section dsl_increaseApproval.
     ).
 
   Lemma increaseApproval_dsl_sat_spec:
-    forall st env msg this,
-      spec_require (funcspec_increaseApproval _spender _value this env msg) st ->
-      forall st0 result,
-        dsl_exec increaseApproval_dsl st0 st env msg this nil = result ->
-        spec_trans (funcspec_increaseApproval _spender _value this env msg) st (ret_st result) /\
-        spec_events (funcspec_increaseApproval _spender _value this env msg) (ret_st result) (ret_evts result).
+    dsl_sat_spec (mc_increaseApproval _spender _value)
+                 increaseApproval_dsl
+                 (funcspec_increaseApproval _spender _value).
   Proof.
-    intros st env msg this Hreq st0 result Hexec.
+    intros st env msg this Hfunc Hreq st0 result Hexec.
+
+    apply increaseApproval_value_inrange in Hfunc.
+    destruct Hfunc as [_ Hvalue].
 
     simpl in Hreq.
     destruct Hreq as [Hpaused Hallowed].
@@ -1485,7 +1489,6 @@ Section dsl_increaseApproval.
     rewrite (spender_immutable _ _ _) in Hexec.
     rewrite (value_immutable _ _ _) in Hexec.
     rewrite (max_uint256_immutable _ _ _) in Hexec.
-    destruct value_in_range as [_ Hvalue].
     rewrite (minus_safe _ _ Hvalue) in Hexec.
     rewrite Hallowed in Hexec; simpl in Hexec.
 
@@ -1499,12 +1502,16 @@ Section dsl_increaseApproval.
   (* If no require can be satisfied, increaseApproval() must revert to the initial state *)
   Lemma increaseApproval_dsl_revert:
     forall st env msg this,
+      m_func msg = mc_increaseApproval _spender _value ->
       ~ spec_require (funcspec_increaseApproval _spender _value this env msg) st ->
       forall st0 result,
         dsl_exec increaseApproval_dsl st0 st env msg this nil = result ->
         result = Stop st0 (ev_revert this :: nil).
   Proof.
-    intros st env msg this Hreq_neg st0 result Hexec.
+    intros st env msg this Hfunc Hreq_neg st0 result Hexec.
+
+    apply increaseApproval_value_inrange in Hfunc.
+    destruct Hfunc as [_ Hvalue].
 
     simpl in Hreq_neg.
     assert (Hreq_impl: st_paused st = ofalse ->
@@ -1529,7 +1536,6 @@ Section dsl_increaseApproval.
       rewrite (spender_immutable _ _ _) in Hexec.
       rewrite (value_immutable _ _ _) in Hexec.
       rewrite (max_uint256_immutable _ _ _) in Hexec.
-      destruct value_in_range as [_ Hvalue].
       rewrite (minus_safe _ _ Hvalue) in Hexec.
       rewrite Hreq_impl in Hexec; simpl in Hexec.
 
@@ -1563,7 +1569,6 @@ Section dsl_decreaseApproval.
   (* Arguments are immutable, generated from solidity *)
   Context `{spender_immutable: forall st env msg, spender st env msg = _spender}.
   Context `{value_immutable: forall st env msg, value st env msg = _value}.
-  Context `{value_in_range: (0 <= _value /\ _value <= MAX_UINT256)%nat}.
   Context `{max_uint256_immutable: forall st env msg, max_uint256 st env msg = MAX_UINT256}.
 
   (* DSL representation of constructor, generated from solidity *)
@@ -1580,14 +1585,11 @@ Section dsl_decreaseApproval.
     ).
 
   Lemma decreaseApproval_dsl_sat_spec_1:
-    forall st env msg this,
-      spec_require (funcspec_decreaseApproval_1 _spender _value this env msg) st ->
-      forall st0 result,
-        dsl_exec decreaseApproval_dsl st0 st env msg this nil = result ->
-        spec_trans (funcspec_decreaseApproval_1 _spender _value this env msg) st (ret_st result) /\
-        spec_events (funcspec_decreaseApproval_1 _spender _value this env msg) (ret_st result) (ret_evts result).
+    dsl_sat_spec (mc_decreaseApproval _spender _value)
+                 decreaseApproval_dsl
+                 (funcspec_decreaseApproval_1 _spender _value).
   Proof.
-    intros st env msg this Hreq st0 result Hexec.
+    intros st env msg this Hfunc Hreq st0 result Hexec.
 
     simpl in Hreq.
     destruct Hreq as [Hpaused Hallowed].
@@ -1610,14 +1612,11 @@ Section dsl_decreaseApproval.
   Qed.
 
   Lemma decreaseApproval_dsl_sat_spec_2:
-    forall st env msg this,
-      spec_require (funcspec_decreaseApproval_2 _spender _value this env msg) st ->
-      forall st0 result,
-        dsl_exec decreaseApproval_dsl st0 st env msg this nil = result ->
-        spec_trans (funcspec_decreaseApproval_2 _spender _value this env msg) st (ret_st result) /\
-        spec_events (funcspec_decreaseApproval_2 _spender _value this env msg) (ret_st result) (ret_evts result).
+    dsl_sat_spec (mc_decreaseApproval _spender _value)
+                 decreaseApproval_dsl
+                 (funcspec_decreaseApproval_2 _spender _value).
   Proof.
-    intros st env msg this Hreq st0 result Hexec.
+    intros st env msg this Hfunc Hreq st0 result Hexec.
 
     simpl in Hreq.
     destruct Hreq as [Hpaused Hallowed].
@@ -1643,13 +1642,14 @@ Section dsl_decreaseApproval.
   (* If no require can be satisfied, decreaseApproval() must revert to the initial state *)
   Lemma decreaseApproval_dsl_revert:
     forall st env msg this,
+      m_func msg = mc_decreaseApproval _spender _value ->
       ~ spec_require (funcspec_decreaseApproval_1 _spender _value this env msg) st ->
       ~ spec_require (funcspec_decreaseApproval_2 _spender _value this env msg) st ->
       forall st0 result,
         dsl_exec decreaseApproval_dsl st0 st env msg this nil = result ->
         result = Stop st0 (ev_revert this :: nil).
   Proof.
-    intros st env msg this Hreq_1 Hreq_2 st0 result Hexec.
+    intros st env msg this Hfunc Hreq_1 Hreq_2 st0 result Hexec.
 
     simpl in Hreq_1.
     assert (Hreq1_impl: st_paused st = ofalse ->
